concurrency/compiler/concurrent_compiler_safety_proof.v
@@ -1,10 +1,14 @@
 
+Require Import VST.concurrency.common.HybridMachineSig.
+Import HybridMachineSig.
+
 Require Import VST.concurrency.compiler.concurrent_compiler_simulation.
 Require Import VST.concurrency.compiler.concurrent_compiler_simulation_proof.
 Require Import VST.concurrency.compiler.sequential_compiler_correct.
 Require Import VST.concurrency.compiler.concurrent_compiler_safety.
 Require Import VST.concurrency.compiler.concurrent_compiler_simulation_proof.
 Require Import VST.concurrency.compiler.safety_equivalence.
+Require Import VST.concurrency.compiler.HybridMachine_simulation.
 
 
 (*Clight Machine *)
@@ -28,59 +32,110 @@ Module Concurrent_Safety (CC_correct: CompCert_correctness).
     Definition Asm_init_state (p: Asm.program):=
     Asm.entry_point (@the_ge p).
   
-  Search semantics.Semantics.
-  Lemma ConcurrentCompilerSafety:
-    forall (p : Clight.program) (tp : Asm.program),
-       CC_correct.CompCert_compiler p = Some tp ->
-       forall asm_genv_safety : Asm_core.safe_genv (@the_ge tp),
-         let SemSource:= (ClightSemantincsForMachines.ClightSem (Clight.globalenv p)) in
+    Search semantics.Semantics.
+
+
+    
+    Lemma explicit_safety_step:
+      forall (p : Clight.program) (tp : Asm.program) (asm_genv_safety : Asm_core.safe_genv the_ge),
+        let SemSource:= (ClightSemantincsForMachines.ClightSem (Clight.globalenv p)) in
          let SemTarget:= @X86Sem tp asm_genv_safety in
-    concurrent_simulation_safety_preservation_export 
-      (SemSource:= SemSource)
-      (SourceThreadPool:= threadPool.OrdinalPool.OrdinalThreadPool(Sem:=SemSource))
-      (SourceMachineSig:= HybridMachine.DryHybridMachine.DryHybridMachineSig)
-      (SemTarget :=  SemTarget)
-      (TargetThreadPool:= threadPool.OrdinalPool.OrdinalThreadPool(Sem:=SemTarget))
-      (TargetMachineSig:= HybridMachine.DryHybridMachine.DryHybridMachineSig)
-      (Clight_init_state p)
-      (Asm_init_state tp)
-  .
-    unfold concurrent_simulation_safety_preservation_export; intros.
-    pose proof (ConcurrentCompilerCorrectness p tp H asm_genv_safety U) as HH.
-    unfold ConcurrentCompilerCorrectness_specification in *.
-    (*exploratory*)
-    pose proof (HybridMachine_simulation.initial_setup HH) as INIT.
-    simpl in INIT.
-    unfold HybridMachineSig.HybridMachineSig.init_machine' in INIT.
-    assert (tpool: @OrdinalPool.t HybridMachine.DryHybridMachine.dryResources
-    (@DSem (Clight.globalenv p))) by admit.
-    specialize (INIT (@the_ge tp)(Clight.globalenv p) init_thread init_mem_source
-                     init_mem_source main args tpool
-                     (Some (permissions.getCurPerm init_mem_source, permissions.empty_map))).
-    simpl in *.
-    unfold HybridMachine.DryHybridMachine.init_mach in *.
-    simpl in *.
-    match type of INIT with
-      | ?A -> ?B => assert A
-    end.
-    admit.
-    specialize (INIT H2).
-    match type of INIT with
-      | ?A -> ?B => assert A
-    end.
-    eexists.
+         forall (U : schedule) (m_s m_t : Memory.Mem.mem)
+             (j : Values.Val.meminj) (c : Asm.state)
+             (C_source : OrdinalPool.t(Sem:=SemSource))
+             (C_target : OrdinalPool.t(Sem:=SemTarget)) tr
+             (SIM : HybridMachine_simulation (ClightConcurSem U)
+                                             (AsmConcurSem U)) (cd : index SIM),
+           match_state SIM cd j C_source m_s C_target
+                    m_t ->
+        (forall U,
+            explicit_safety
+              HybridMachine.DryHybridMachine.dryResources
+              SemSource
+              (threadPool.OrdinalPool.OrdinalThreadPool(Sem:=SemSource))
+              HybridMachine.DryHybridMachine.DryHybridMachineSig
+              U tr C_source m_s) ->
+        forall U,
+            explicit_safety
+              HybridMachine.DryHybridMachine.dryResources
+              SemTarget
+              (threadPool.OrdinalPool.OrdinalThreadPool(Sem:=SemTarget))
+              HybridMachine.DryHybridMachine.DryHybridMachineSig
+              U tr C_target m_t.
+    Proof.
+    Admitted.
+
+
+
+    Lemma csafety_step:
+      forall (p : Clight.program) (tp : Asm.program) (asm_genv_safety : Asm_core.safe_genv the_ge),
+        let SemSource:= (ClightSemantincsForMachines.ClightSem (Clight.globalenv p)) in
+         let SemTarget:= @X86Sem tp asm_genv_safety in
+         forall (U : schedule) (init_mem_source' : Memory.Mem.mem)
+             (j : Values.Val.meminj) (c : Asm.state)
+             (C_source : OrdinalPool.t(Sem:=SemSource))
+             (C_target : OrdinalPool.t) tr
+             (SIM : HybridMachine_simulation (ClightConcurSem U)
+                                             (AsmConcurSem U)) (cd : index SIM),
+        match_state SIM cd j C_source init_mem_source' C_target
+                    (Asm.get_mem c) ->
+        (forall n : nat,
+            HybridCoarseMachine.csafe(Sem:=SemSource)
+                                     (resources:=HybridMachine.DryHybridMachine.dryResources)
+                                     (ThreadPool:= threadPool.OrdinalPool.OrdinalThreadPool(Sem:=SemSource))
+      (machineSig:= HybridMachine.DryHybridMachine.DryHybridMachineSig)
+                                     (U, tr, C_source)
+                                      init_mem_source' n) ->
+        forall n : nat,
+          HybridCoarseMachine.csafe (Sem:=SemTarget)
+                                     (resources:=HybridMachine.DryHybridMachine.dryResources)
+                                     (ThreadPool:= threadPool.OrdinalPool.OrdinalThreadPool(Sem:=SemTarget))
+      (machineSig:= HybridMachine.DryHybridMachine.DryHybridMachineSig)
+                                     (U, tr, C_target)
+                                     (Asm.get_mem c) n.
+    Proof.
+      intros.
+      eapply explicit_safety_csafe; eauto; intros.
+      - admit. (*Initial scheudle is valid. *)
+      - eapply explicit_safety_step in H; eauto.
+        eapply csafe_explicit_safety; simpl.
+        
+        
+    Admitted.
+
+
     
-    unfold HH.
-    
-    
-    assert (HybridMachine_simulation.initial_source_thread
-              HH init_mem_source init_thread main args).
-    simpl.
-    eapply HybridMachine_simulation.initial_setup in H0.
- 
-      (ConcurrentCompilerCorrectness_specification
-            (Clight.globalenv p) tp asm_genv_safety).
-    
-  Admitted.
+    Lemma ConcurrentCompilerSafety:
+      forall (p : Clight.program) (tp : Asm.program),
+        CC_correct.CompCert_compiler p = Some tp ->
+        forall asm_genv_safety : Asm_core.safe_genv (@the_ge tp),
+          let SemSource:= (ClightSemantincsForMachines.ClightSem (Clight.globalenv p)) in
+          let SemTarget:= @X86Sem tp asm_genv_safety in
+          concurrent_simulation_safety_preservation 
+            (SemSource:= SemSource)
+            (SourceThreadPool:= threadPool.OrdinalPool.OrdinalThreadPool(Sem:=SemSource))
+            (SourceMachineSig:= HybridMachine.DryHybridMachine.DryHybridMachineSig)
+            (SemTarget :=  SemTarget)
+            (TargetThreadPool:= threadPool.OrdinalPool.OrdinalThreadPool(Sem:=SemTarget))
+            (TargetMachineSig:= HybridMachine.DryHybridMachine.DryHybridMachineSig)
+    .
+      unfold concurrent_simulation_safety_preservation; intros.
+      pose proof (ConcurrentCompilerCorrectness p tp H asm_genv_safety U) as SIM.
+
+      (*Construct the initial state*)
+      
+      apply (HybridMachine_simulation.initial_setup SIM) in H0 as
+          (j&cd&t_mach_state&t_mem&t_mem'&r2&INIT&?).
+      assert(INIT':= INIT).
+      destruct r2; try solve[inversion INIT'].
+      destruct INIT' as (c&?&?).
+      subst t_mach_state; simpl in *.
+      do 3 eexists; split; eauto.
+      destruct H2 as (H21 & H22); subst.
+      clear INIT H21.
+
+      (* Step preserves safety*)
+      eapply safety_step; try eapply H0; eauto.
+    Qed.
       
 End Concurrent_Safety.
